Finish the walkthrough of Chapter 1

hello.lean
@@ -1,15 +1,23 @@
-set_option trace.debug.eqn_compiler true
 set_option trace.cc true
 set_option trace.debug.dsimplify true
 set_option trace.simplify.context true
 set_option trace.simplify.rewrite true
-set_option trace.debug true
+-- set_option trace.debug.eqn_compiler true
+-- set_option trace.debug true
+
+-- Adapted from the default code 
+-- on https://leanprover.github.io/live/latest/
 
 lemma ℕ_addition_commutative
 (n m : ℕ) : 
     n + m = m + n :=
 by cc
 -- TODO why simp failed?
+
+-- The following are adapted from 
+-- Chapter 1, The Hitchhiker’s Guide to Logical Verification
+
+-- 1.1.2 Terms
 
 lemma function_currying_right_associative
 (σ τ ν : Type) : 
@@ -51,11 +59,15 @@ constants trool.true trool.false trool.maybe : trool
 
 #check trool.maybe
 
+-- 1.2.1 Natural Numbers
+
 inductive ℕat : Type
 | zero : ℕat
 | succ : ℕat → ℕat
 
 #print ℕat
+
+-- 1.2.2 Arithmetic Expressions & 1.3 Function Definitions
 
 inductive ArithmeticExpr : Type
 | num : ℤ → ArithmeticExpr
@@ -73,8 +85,16 @@ def eval (env : string → ℤ) : ArithmeticExpr → ℤ
 | (ArithmeticExpr.mul e₁ e₂) := eval e₁ * eval e₂
 | (ArithmeticExpr.div e₁ e₂) := eval e₁ / eval e₂
 
-def example_env (key : string) : ℤ
+def example_env₂ (key : string) : ℤ
 := if key = "any" then 100 else string.to_nat key
+
+def example_env : string → ℤ
+| "one" := 1
+| "two" := 2
+| "three" := 3
+| "four" := 4
+| "any" := 100
+| key := string.to_nat key
 
 def example_eval : ℤ
 := (eval example_env) (ArithmeticExpr.sub
@@ -85,7 +105,7 @@ def example_eval : ℤ
         (ArithmeticExpr.num 3)
     )
     (ArithmeticExpr.mul
-        (ArithmeticExpr.num 5) (ArithmeticExpr.sym "4")
+        (ArithmeticExpr.num 5) (ArithmeticExpr.sym "four")
     )
 )
 def expected_eval : ℤ
@@ -98,6 +118,8 @@ apply and.intro,
 refl, -- example_eval = expected_eval
 refl -- example_eval = 14
 end
+
+-- 1.2.5 Lists
 
 inductive List (α : Type) : Type
 | nil : List
@@ -117,3 +139,94 @@ inductive List (α : Type) : Type
     cat :: cats
 #check λ(Animal : Type) (cat_1 cat_ooo cat_n : Animal), 
     cat_1 :: cat_ooo :: cat_n :: []
+
+-- 1.3 Function Definitions
+
+def add : ℕ → ℕ → ℕ
+| m nat.zero := m
+| m (nat.succ n) := nat.succ (add m n)
+
+-- #eval employs an optimized interpreter
+#eval add 2 7
+-- #reduce uses Lean’s inference kernel, which is less efficient
+#reduce add 2 7
+
+def mul : ℕ → ℕ → ℕ
+| _ nat.zero := nat.zero
+| m (nat.succ n) := add m (mul m n)
+
+#eval mul 2 7
+
+def power : ℕ → ℕ → ℕ
+| _ nat.zero := 1
+| m (nat.succ n) := mul m (power m n)
+
+#eval power 2 3
+
+def power₂ (m : ℕ) : ℕ → ℕ
+| nat.zero := 1
+| (nat.succ n) := mul m (power m n)
+
+#eval power₂ 2 3
+
+def iter (α : Type) (z : α) (f : α → α) : ℕ → α
+| nat.zero := z
+| (nat.succ n) := f (iter n)
+
+def power₃ (m n : ℕ) : ℕ
+:= iter ℕ 1 (λl, m * l) n
+
+def list_append (α : Type) : list α → list α → list α
+| list.nil xs := xs
+| (list.cons x xs) ys := list.cons x (list_append xs ys)
+
+#check list_append
+
+#eval list_append _ [3, 1] [4, 1, 5]
+
+def list_append₂ {α : Type} : list α → list α → list α
+| list.nil xs := xs
+| (list.cons x xs) ys := list.cons x (list_append₂ xs ys)
+
+#check list_append₂
+#eval list_append₂ [3, 1] [4, 1, 5]
+
+-- The at sign (@) can be used to make the implicit arguments explicit
+#check @list_append₂
+#eval @list_append₂ ℤ [3, 1] [4, 1, 5]
+#eval @list_append₂ _ [3, 1] [4, 1, 5]
+
+-- We can use syntactic sugar in the definition, both in the patterns
+-- on the left-hand sides of := and in the right-hand sides
+def list_append₃ {α : Type} : list α → list α → list α
+| [] xs := xs
+| (x :: xs) ys := x :: (list_append₃ xs ys)
+
+def reverse {α : Type} : list α → list α
+| [] := []
+| (x :: xs) := (reverse xs) ++ [x]
+
+-- 1.4 Lemma Statements
+
+lemma add_commutative (m n : ℕ) :
+    add m n = add n m :=
+sorry
+
+lemma add_associative (l m n : ℕ) :
+    add (add l m) n = add l (add m n) :=
+sorry
+ 
+lemma mul_commutative (m n : ℕ) :
+    mul m n = mul n m :=
+sorry
+
+lemma mul_add_distributive (l m n : ℕ) :
+    mul l (add m n) = add (mul l m) (mul l n) :=
+sorry
+
+lemma reverse_reverse {α : Type} (xs : list α) :
+    reverse (reverse xs) = xs :=
+sorry
+
+axiom a_less_b :
+    a < b
